RGA -set

inductive_proof/RGA_set_pre-cond/App_do_pre_first.fst
@@ -2,20 +2,21 @@ module App_do_pre_first
 
 module S = Set_extended
 
-// the set has entries with unique timestamps
+// the set has entries with unique timestamps 
 let unique_st (s:S.set (nat & (nat & nat))) =
   S.forall_s s (fun e -> not (S.exists_s s (fun e1 -> snd e <> snd e1 && fst e = fst e1)))
 
+let mem_id_s (id:nat) (s:S.set (nat & (nat & nat))) 
+  : (r:bool {s = S.empty ==> r == false}) =
+  S.exists_s s (fun e -> fst e = id)
+
 #set-options "--query_stats"
 // the concrete state type
-type concrete_st = s:(S.set (nat & (nat & nat)) & S.set nat) {unique_st (fst s)}
+type concrete_st = s:(S.set (nat & (nat & nat)) & S.set nat) {unique_st (fst s) /\
+                                                      (forall id. S.mem id (snd s) ==> mem_id_s id (fst s))}
                    // first ele of the pair is a tuple of timestamp, 
                    //     id after which the ele is to be inserted and ele to be inserted
                    // second ele of the pair is a tombstone set
-
-let mem_id_s (id:nat) (s:S.set (nat & (nat & nat))) 
-  : (r:bool {s = S.empty ==> r == false}) =
-  S.exists_s s (fun e -> fst e = id) //exists e. S.mem e s /\ fst e = id
 
 // init state
 let init_st = (S.empty, S.empty)
@@ -50,22 +51,24 @@ let get_ele (op:op_t{Add_after? (snd op)}) : nat =
 let get_after_id (op:op_t{Add_after? (snd op)}) : nat =
   let (_, Add_after id _) = op in id
 
-let get_rem_id (op:op_t{Remove? (snd op)}) : nat =
+let get_rem_id (op:op_t{Remove? (snd op)}) : pos =
   let (_, Remove id) = op in id
 
-let do_pre (s:concrete_st) (op:op_t) =
+let do_pre (s:concrete_st) (op:op_t) : prop =
   match op with
-  |(ts, Add_after after_id ele) -> ~ (mem_id_s ts (fst s) \/ S.mem ts (snd s)) /\                                
-                                  (~ (after_id = 0) ==> mem_id_s after_id (fst s))
-  |(_, Remove id) -> mem_id_s id (fst s) /\ ~ (S.mem id (snd s))
+  |(ts, Add_after after_id ele) -> ~ (mem_id_s ts (fst s))                               
+                                  //(~ (after_id = 0) ==> mem_id_s after_id (fst s))
+  |(_, Remove id) -> True //if mem_id_s id (fst s) then True else False ///\ ~ (S.mem id (snd s))
 
 // apply an operation to a state
 let do (s:concrete_st) (op:op_t{do_pre s op}) 
-  : (r:concrete_st{(Add_after? (snd op) ==> (forall id. mem_id_s id (fst r) <==> mem_id_s id (fst s) \/ id = fst op)) /\
-                   (Remove? (snd op) ==> (forall id. S.mem id (snd r) <==> S.mem id (snd s) \/ id = get_rem_id op))}) =
+  : (r:concrete_st{//(Add_after? (snd op) ==> (forall id. mem_id_s id (fst r) <==> mem_id_s id (fst s) \/ id = fst op)) /\
+                   //(Remove? (snd op) ==> (forall id. S.mem id (snd r) <==> S.mem id (snd s) \/ id = get_rem_id op)) /\
+                   S.subset (fst s) (fst r) /\ S.subset (snd s) (snd r)}) =
    match op with
-  |(ts, Add_after after_id ele) -> (S.add (ts, (after_id, ele)) (fst s), snd s)
-  |(_, Remove id) -> (fst s, S.add id (snd s))
+  |(ts, Add_after after_id ele) -> if (after_id <> 0 && not (mem_id_s after_id (fst s))) then s 
+                                  else (S.add (ts, (after_id, ele)) (fst s), snd s)
+  |(_, Remove id) -> if mem_id_s id (fst s) (*&& not (S.mem id (snd s))*) then (fst s, S.add id (snd s)) else s
   
 let lem_do (a b:concrete_st) (op:op_t)
    : Lemma (requires eq a b /\ do_pre a op)
@@ -80,14 +83,14 @@ let resolve_conflict (x:op_t) (y:op_t{fst x <> fst y}) : resolve_conflict_res =
   |(ts1, (Add_after id1 _)), (ts2, (Add_after id2 _)) -> if id1 = id2 then 
                                                            if ts1 > ts2 then First_then_second else Second_then_first 
                                                         else First_then_second //ts1 <> id2 /\ ts2 <> id1
-  |(ts1, (Add_after id1 _)), (ts2, Remove id2) -> if id1 = id2 then Second_then_first else First_then_second //ts1 <> id2
+  |(ts1, (Add_after id1 _)), (ts2, Remove id2) -> if ts1 = id2 then Second_then_first else First_then_second //ts1 <> id2
   |(ts1, Remove id1), (ts2, (Add_after id2 _)) -> First_then_second //ts2 <> id1
-  |(ts1, Remove id1), (ts2, Remove id2) -> if id1 = id2 then First else First_then_second
+  |(ts1, Remove id1), (ts2, Remove id2) -> (*if id1 = id2 then First else*) First_then_second
 
 // concrete merge pre-condition
 let merge_pre l a b = 
-  S.subset (fst l) (fst a) /\ S.subset (fst l) (fst b) /\
-  S.subset (snd l) (snd a) /\ S.subset (snd l) (snd b) /\
+  //S.subset (fst l) (fst a) /\ S.subset (fst l) (fst b) /\
+  //S.subset (snd l) (snd a) /\ S.subset (snd l) (snd b) /\
   (forall id. mem_id_s id (fst l) ==> ~ (mem_id_s id (S.difference (fst a) (fst l)))) /\
   (forall id. mem_id_s id (fst l) ==> ~ (mem_id_s id (S.difference (fst b) (fst l)))) /\
   (forall id. mem_id_s id (S.difference (fst a) (fst l)) ==> ~ (mem_id_s id (S.difference (fst b) (fst l))))
@@ -97,12 +100,13 @@ let concrete_merge (lca s1:concrete_st) (s2:concrete_st{merge_pre lca s1 s2})
                    (forall e. S.mem e (snd r) <==> S.mem e (snd lca) \/ S.mem e (snd s1) \/ S.mem e (snd s2))}*)) =
   (//S.union (S.intersect (fst s1) (fst s2))
   
-   S.union (fst lca)
-           (S.union (S.difference (fst s1) (fst lca)) (S.difference (fst s2) (fst lca))),
+   (*S.union (fst lca)
+           (S.union (S.difference (fst s1) (fst lca)) (S.difference (fst s2) (fst lca))),*)
+   S.union (fst lca) (S.union (fst s1) (fst s2)),
    
    S.union (snd lca) (S.union (snd s1) (snd s2)))
   
-  //(S.union (fst s1) (fst s2), (S.union (snd s1) (snd s2)))
+   //S.union (fst s1) (fst s2), (S.union (snd s1) (snd s2)))
   
 // Prove that merge is commutative
 let merge_is_comm (lca s1 s2:st)
@@ -111,7 +115,7 @@ let merge_is_comm (lca s1 s2:st)
           (ensures merge_pre (v_of lca) (v_of s2) (v_of s1) /\
                    (eq (concrete_merge (v_of lca) (v_of s1) (v_of s2)) 
                        (concrete_merge (v_of lca) (v_of s2) (v_of s1)))) = ()           
-                       
+                      
 let linearizable_s1_0''_base_base (lca s1 s2':st) (last2:op_t)
   : Lemma (requires do_pre (v_of s2') last2 /\
                     consistent_branches lca s1 (do_st s2' last2) /\
@@ -121,58 +125,17 @@ let linearizable_s1_0''_base_base (lca s1 s2':st) (last2:op_t)
         
           (ensures eq (do (v_of s2') last2) (concrete_merge (v_of lca) (v_of s1) (do (v_of s2') last2))) = ()
 
-let linearizable_s1_0''_base (lca s1 s2':st) (last2:op_t)
+#push-options "--z3rlimit 100"
+let linearizable_s1_0''_base_do_pre (lca s1 s2':st) (last2:op_t)
   : Lemma (requires do_pre (v_of s2') last2 /\ 
                     consistent_branches lca s1 (do_st s2' last2) /\
                     ops_of s1 == ops_of lca /\ ops_of s2' == ops_of lca /\
-                    fst last2 > 0)
-          (ensures eq (do (v_of s2') last2) (concrete_merge (v_of lca) (v_of s1) (do (v_of s2') last2))) = () //extra
-
-#push-options "--z3rlimit 50"
-let linearizable_s1_0'1 (lca s1 s2:st)
-  : Lemma (requires consistent_branches lca s1 s2 /\
-                    length (ops_of s2) > length (ops_of lca) /\
-                    ops_of s1 = ops_of lca /\
-                    merge_pre (v_of lca) (v_of s1) (v_of s2))
-          (ensures eq (v_of s2) (concrete_merge (v_of lca) (v_of s1) (v_of s2))) = ()
-          
-let rec linearizable_s1_0''_base_do_pre1 (lca s1 s2':st) (last2:op_t)
-  : Lemma (requires do_pre (v_of s2') last2 /\ 
-                    consistent_branches lca s1 (do_st s2' last2) /\
-                    ops_of s1 == ops_of lca /\ ops_of s2' == ops_of lca /\
-                    fst last2 > 0 /\ Remove? (snd last2) /\
+                    fst last2 > 0 /\
                     length (ops_of s2') > 0)
-          (ensures do_pre (v_of (inverse_st s2')) last2) 
-          (decreases length (ops_of s2')) =
-  if length (ops_of s2') = 0 then ()
-  else 
-    (lem_apply_log init_st (ops_of s2');
-     let _, lastop = un_snoc (ops_of s2') in
-     let s2'' = inverse_st s2' in
-     if Remove? (snd lastop) then () 
-     else 
-       (if fst lastop <> get_rem_id last2 then () 
-        else 
-          (admit();assert (~ (S.mem (get_rem_id last2) (snd (v_of s2''))));
-           assume (mem_id_s (get_rem_id last2) (fst (v_of s2'')));
-           ())))
-
-  (*if length (ops_of lca) = 0 then admit()
-  else if length (ops_of lca) = 1 then 
-    (lem_apply_log init_st (ops_of s2');
-     let _, lastop = un_snoc (ops_of s2') in
-     //inverse_helper init_st (ops_of lca) lastop;
-     
-     //if Add_after? (snd lastop) then admit() else ())
-     assert (fst init_st == S.empty); 
-     assert (not (mem_id_s (fst last2) (fst init_st))); 
-     if Remove? (snd last2) then () else ())
-  else 
-    (let l' = inverse_st lca in
-     assume (do_pre (v_of l') last2 /\
-             length (ops_of l') > 0 /\
-             consistent_branches l' l' (do_st l' last2));
-     linearizable_s1_0''_base_do_pre l' l' l' last2); ()*)
+          (ensures do_pre (v_of (inverse_st s2')) last2) = 
+  lem_apply_log init_st (ops_of s2');
+  let pre, lastop = un_snoc (ops_of s2') in
+  inverse_helper init_st pre lastop
 
 let linearizable_s1_0''_base_merge_pre (lca s1 s2':st) (last2:op_t)
   : Lemma (requires do_pre (v_of s2') last2 /\ 
@@ -211,8 +174,9 @@ let linearizable_s1_0''_do_pre (lca s1 s2':st) (last2:op_t)
                     ops_of s1 = ops_of lca /\                    
                     fst last2 > 0 /\
                     length (ops_of s2') > length (ops_of lca))         
-          (ensures do_pre (v_of (inverse_st s2')) last2) = admit()
+          (ensures do_pre (v_of (inverse_st s2')) last2) = ()
 
+//#push-options "--z3rlimit 200"
 let linearizable_s1_0''_merge_pre (lca s1 s2':st) (last2:op_t)
   : Lemma (requires do_pre (v_of s2') last2 /\
                     consistent_branches lca s1 (do_st s2' last2) /\
@@ -248,6 +212,240 @@ let linearizable_s1_0_s2_0_base (lca s1 s2:st)
         
           (ensures eq (v_of lca) (concrete_merge (v_of lca) (v_of s1) (v_of s2))) = ()
 
+let linearizable_gt0_base_fts (lca s1 s2:st) (last1 last2:op_t)
+  : Lemma (requires do_pre (v_of s1) last1 /\ do_pre (v_of s2) last2 /\ 
+                    consistent_branches lca (do_st s1 last1) (do_st s2 last2) /\
+                    consistent_branches lca s1 s2 /\
+                    ops_of s1 = ops_of lca /\ ops_of s2 = ops_of lca /\
+                    fst last1 <> fst last2 /\
+                    merge_pre (v_of lca) (do (v_of s1) last1) (do (v_of s2) last2) /\
+                    First_then_second? (resolve_conflict last1 last2) /\
+                    Remove? (snd last1) /\ Add_after? (snd last2) /\
+                    merge_pre (v_of lca) (v_of s1) (do (v_of s2) last2) /\
+                    do_pre (concrete_merge (v_of lca) (v_of s1) (do (v_of s2) last2)) last1)
+         
+          (ensures //merge_pre (v_of lca) (v_of s1) (do (v_of s2) last2) (*/\
+                   //do_pre (concrete_merge (v_of lca) (v_of s1) (do (v_of s2) last2)) last1 /\
+                   eq (do (concrete_merge (v_of lca) (v_of s1) (do (v_of s2) last2)) last1)
+                      (concrete_merge (v_of lca) (do (v_of s1) last1) (do (v_of s2) last2))) = 
+  (*assume ((Remove? (snd last1) /\ Add_after? (snd last2) ==> fst last2 <> get_rem_id last1) /\
+          (Add_after? (snd last1) /\ Add_after? (snd last2) /\ get_after_id last1 <> get_after_id last2 ==>
+                      fst last1 <> get_after_id last2 /\ fst last2 <> get_after_id last1));*)
+  assert (~ (mem_id_s (fst last2) (fst (v_of lca))));
+  //assert (~ (mem_id_s (fst last2) (concrete_merge (v_of lca) (v_of s1) (do (v_of s2) last2))));
+  //assume (fst last2 <> get_rem_id last1);
+  ()
+
+
+
+
+
+
+
+
+
+
+
+
+
+let linearizable_s1_0' (lca s1 s2:st)
+  : Lemma (requires consistent_branches lca s1 s2 /\
+                    merge_pre (v_of lca) (v_of s1) (v_of s2) /\
+                    length (ops_of s2) > length (ops_of lca) /\
+                    ops_of s1 = ops_of lca)
+          (ensures eq (v_of s2) (concrete_merge (v_of lca) (v_of s1) (v_of s2))) = ()
+
+
+let linearizable_gt0_fts (lca s1 s2:st)
+  : Lemma (requires consistent_branches_s1s2_gt0 lca s1 s2 /\
+                    consistent_branches lca (inverse_st s1) s2 /\
+                    consistent_branches lca (inverse_st s1) (inverse_st s2) /\
+                    (let _, last1 = un_snoc (ops_of s1) in
+                    let _, last2 = un_snoc (ops_of s2) in
+                    fst last1 <> fst last2 /\
+                    First_then_second? (resolve_conflict last1 last2) /\
+                    merge_pre (v_of lca) (v_of s1) (v_of s2) /\
+                    merge_pre (v_of lca) (v_of (inverse_st s1)) (v_of s2) /\
+                    do_pre (concrete_merge (v_of lca) (v_of (inverse_st s1)) (v_of s2)) last1))
+          (ensures (let _, last1 = un_snoc (ops_of s1) in
+                    (*merge_pre (v_of lca) (v_of (inverse_st s1)) (v_of s2) /\
+                    do_pre (concrete_merge (v_of lca) (v_of (inverse_st s1)) (v_of s2)) last1 /\*)
+                    eq (do (concrete_merge (v_of lca) (v_of (inverse_st s1)) (v_of s2)) last1)
+                       (concrete_merge (v_of lca) (v_of s1) (v_of s2)))) = ()
+                        
+
+let linearizable_gt0_base_fts (lca s1 s2:st) (last1 last2:op_t)
+  : Lemma (requires do_pre (v_of s1) last1 /\ do_pre (v_of s2) last2 /\ 
+                    consistent_branches lca (do_st s1 last1) (do_st s2 last2) /\
+                    consistent_branches lca s1 s2 /\
+                    ops_of s1 = ops_of lca /\ ops_of s2 = ops_of lca /\
+                    fst last1 <> fst last2 /\
+                    merge_pre (v_of lca) (do (v_of s1) last1) (do (v_of s2) last2) /\
+                    First_then_second? (resolve_conflict last1 last2) /\
+                    merge_pre (v_of lca) (v_of s1) (do (v_of s2) last2) /\
+                    do_pre (concrete_merge (v_of lca) (v_of s1) (do (v_of s2) last2)) last1)
+         
+          (ensures //merge_pre (v_of lca) (v_of s1) (do (v_of s2) last2) /\
+                   //do_pre (concrete_merge (v_of lca) (v_of s1) (do (v_of s2) last2)) last1 /\
+                   eq (do (concrete_merge (v_of lca) (v_of s1) (do (v_of s2) last2)) last1)
+                      (concrete_merge (v_of lca) (do (v_of s1) last1) (do (v_of s2) last2))) = () 
+
+
+#push-options "--z3rlimit 100"
+(*let linearizable_s1_0'1 (lca s1 s2:st)
+  : Lemma (requires consistent_branches lca s1 s2 /\
+                    length (ops_of s2) > length (ops_of lca) /\
+                    ops_of s1 = ops_of lca /\
+                    merge_pre (v_of lca) (v_of s1) (v_of s2))
+          (ensures eq (v_of s2) (concrete_merge (v_of lca) (v_of s1) (v_of s2))) = admit()
+
+#push-options "--z3rlimit 200"
+let linearizable_gt0_s21 (lca s1 s2:st)
+  : Lemma (requires consistent_branches_s1s2_gt0 lca s1 s2 /\
+                    consistent_branches lca s1 (inverse_st s2) /\
+                    consistent_branches lca (inverse_st s1) (inverse_st s2) /\
+                    (let _, last1 = un_snoc (ops_of s1) in
+                    let _, last2 = un_snoc (ops_of s2) in
+                    merge_pre (v_of lca) (v_of s1) (v_of (inverse_st s2)) /\ 
+                    fst last1 <> fst last2 /\
+                    Second_then_first? (resolve_conflict last1 last2)) /\
+                    merge_pre (v_of lca) (v_of s1) (v_of s2))
+          (ensures (let pre2, last2 = un_snoc (ops_of s2) in 
+                    //merge_pre (v_of lca) (v_of s1) (v_of (inverse_st s2)) /\
+                    do_pre (concrete_merge (v_of lca) (v_of s1) (v_of (inverse_st s2))) last2 (*/\
+                    eq (do (concrete_merge (v_of lca) (v_of s1) (v_of (inverse_st s2))) last2)
+                       (concrete_merge (v_of lca) (v_of s1) (v_of s2)*))) =
+  lem_apply_log init_st (ops_of s2);
+  let pre2, last2 = un_snoc (ops_of s2) in 
+  inverse_helper init_st pre2 last2;
+  assert (v_of s2 = do (v_of (inverse_st s2)) last2);
+  if Remove? (snd last2) then () else ()*)
+
+let rec linearizable_s1_0''_base_do_pre1 (lca s1 s2':st) (last2:op_t)
+  : Lemma (requires do_pre (v_of s2') last2 /\ 
+                    consistent_branches lca s1 (do_st s2' last2) /\
+                    ops_of s1 == ops_of lca /\ ops_of s2' == ops_of lca /\
+                    fst last2 > 0 /\ //Add_after? (snd last2) /\
+                    length (ops_of s2') > 0)
+          (ensures do_pre (v_of (inverse_st s2')) last2) 
+          (decreases length (ops_of s2')) =
+  lem_apply_log init_st (ops_of s2');
+  let pre, lastop = un_snoc (ops_of s2') in
+  inverse_helper init_st pre lastop;
+  (*if length (ops_of s2') = 0 then ()
+  else 
+    (lem_apply_log init_st (ops_of s2');
+     let _, lastop = un_snoc (ops_of s2') in
+     let s2'' = inverse_st s2' in
+     if Remove? (snd lastop) then () 
+     else 
+       (if fst lastop <> get_rem_id last2 then () 
+        else 
+          (();//assert (~ (S.mem (get_rem_id last2) (snd (v_of s2''))));
+           //assume (mem_id_s (get_rem_id last2) (fst (v_of s2'')));
+           ())))*) ()
+
+  (*if length (ops_of lca) = 0 then admit()
+  else if length (ops_of lca) = 1 then 
+    (lem_apply_log init_st (ops_of s2');
+     let _, lastop = un_snoc (ops_of s2') in
+     //inverse_helper init_st (ops_of lca) lastop;
+     
+     //if Add_after? (snd lastop) then admit() else ())
+     assert (fst init_st == S.empty); 
+     assert (not (mem_id_s (fst last2) (fst init_st))); 
+     if Remove? (snd last2) then () else ())
+  else 
+    (let l' = inverse_st lca in
+     assume (do_pre (v_of l') last2 /\
+             length (ops_of l') > 0 /\
+             consistent_branches l' l' (do_st l' last2));
+     linearizable_s1_0''_base_do_pre l' l' l' last2); ()*)
+
+let linearizable_s1_0''_do_pre1 (lca s1 s2':st) (last2:op_t)
+  : Lemma (requires do_pre (v_of s2') last2 /\
+                    consistent_branches lca s1 (do_st s2' last2) /\
+                    is_prefix (ops_of lca) (ops_of s2') /\
+                    ops_of s1 = ops_of lca /\                    
+                    fst last2 > 0 /\
+                    length (ops_of s2') > length (ops_of lca))         
+          (ensures do_pre (v_of (inverse_st s2')) last2) = ()
+          
+let linearizable_s1_0''_base_merge_pre1 (lca s1 s2':st) (last2:op_t)
+  : Lemma (requires do_pre (v_of s2') last2 /\ 
+                    consistent_branches lca s1 (do_st s2' last2) /\
+                    ops_of s1 == ops_of lca /\ ops_of s2' == ops_of lca /\
+                    fst last2 > 0 /\
+                    merge_pre (v_of lca) (v_of s1) (do (v_of s2') last2) /\
+                    length (ops_of s2') > 0 /\
+                    do_pre (v_of (inverse_st s2')) last2)
+
+          (ensures (let l' = inverse_st lca in
+                    merge_pre (v_of l') (v_of l') (do (v_of l') last2))) = ()
+
+let linearizable_s1_0''_base_ind1 (lca s1 s2':st) (last2:op_t)
+  : Lemma (requires do_pre (v_of s2') last2 /\
+                    consistent_branches lca s1 (do_st s2' last2) /\
+                    ops_of s1 = ops_of lca /\ ops_of s2' = ops_of lca /\
+                    length (ops_of lca) > 0 /\
+
+                    (let l' = inverse_st lca in
+                    let s1' = inverse_st s1 in
+                    let s2'' = inverse_st s2' in
+                    do_pre (v_of s2'') last2 /\ 
+                    consistent_branches l' s1' (do_st s2'' last2) /\
+                    ops_of s1' = ops_of l' /\ ops_of s2'' = ops_of l' /\
+                    merge_pre (v_of l') (v_of s1') (do (v_of s2'') last2) /\
+                    eq (do (v_of s2'') last2) (concrete_merge (v_of l') (v_of s1') (do (v_of s2'') last2))) /\
+                    merge_pre (v_of lca) (v_of s1) (do (v_of s2') last2))
+
+          (ensures eq (do (v_of s2') last2) (concrete_merge (v_of lca) (v_of s1) (do (v_of s2') last2))) = ()
+
+(*let linearizable_s1_0''_do_pre1 (lca s1 s2':st) (last2:op_t)
+  : Lemma (requires do_pre (v_of s2') last2 /\
+                    consistent_branches lca s1 (do_st s2' last2) /\
+                    is_prefix (ops_of lca) (ops_of s2') /\
+                    ops_of s1 = ops_of lca /\                    
+                    fst last2 > 0 /\
+                    length (ops_of s2') > length (ops_of lca))         
+          (ensures do_pre (v_of (inverse_st s2')) last2) = admit()*)
+
+let linearizable_s1_0''_merge_pre1 (lca s1 s2':st) (last2:op_t)
+  : Lemma (requires do_pre (v_of s2') last2 /\
+                    consistent_branches lca s1 (do_st s2' last2) /\
+                    ops_of s1 = ops_of lca /\
+                    length (ops_of s2') > length (ops_of lca) /\
+
+                    (let inv2 = inverse_st s2' in
+                    do_pre (v_of inv2) last2 /\
+                    consistent_branches lca s1 (do_st inv2 last2) /\
+                    merge_pre (v_of lca) (v_of s1) (do (v_of s2') last2)))
+         
+          (ensures merge_pre (v_of lca) (v_of s1) (do (v_of (inverse_st s2')) last2)) = ()
+
+#push-options "--z3rlimit 50"
+let linearizable_s1_0''_ind1 (lca s1 s2':st) (last2:op_t)
+  : Lemma (requires do_pre (v_of s2') last2 /\
+                    consistent_branches lca s1 (do_st s2' last2) /\
+                    ops_of s1 = ops_of lca /\
+                    length (ops_of s2') > length (ops_of lca) /\
+
+                    (let inv2 = inverse_st s2' in
+                    do_pre (v_of inv2) last2 /\
+                    consistent_branches lca s1 (do_st inv2 last2) /\
+                    merge_pre (v_of lca) (v_of s1) (do (v_of inv2) last2) /\
+                    eq (do (v_of inv2) last2) (concrete_merge (v_of lca) (v_of s1) (do (v_of inv2) last2))) /\
+                    merge_pre (v_of lca) (v_of s1) (do (v_of s2') last2))
+        
+          (ensures eq (do (v_of s2') last2) (concrete_merge (v_of lca) (v_of s1) (do (v_of s2') last2))) = ()
+
+let linearizable_s1_0_s2_0_base1 (lca s1 s2:st)
+  : Lemma (requires consistent_branches lca s1 s2 /\
+                    ops_of s1 == ops_of lca /\ ops_of s2 == ops_of lca /\
+                    merge_pre (v_of lca) (v_of s1) (v_of s2))
+        
+          (ensures eq (v_of lca) (concrete_merge (v_of lca) (v_of s1) (v_of s2))) = ()
+
 #push-options "--z3rlimit 100"
 let linearizable_gt0_base_fts (lca s1 s2:st) (last1 last2:op_t)
   : Lemma (requires do_pre (v_of s1) last1 /\ do_pre (v_of s2) last2 /\ 
@@ -256,14 +454,21 @@ let linearizable_gt0_base_fts (lca s1 s2:st) (last1 last2:op_t)
                     ops_of s1 = ops_of lca /\ ops_of s2 = ops_of lca /\
                     fst last1 <> fst last2 /\
                     merge_pre (v_of lca) (do (v_of s1) last1) (do (v_of s2) last2) /\
-                    First_then_second? (resolve_conflict last1 last2))
+                    First_then_second? (resolve_conflict last1 last2) /\
+                    Remove? (snd last1) /\ Add_after? (snd last2) /\
+                    merge_pre (v_of lca) (v_of s1) (do (v_of s2) last2))
          
-          (ensures merge_pre (v_of lca) (v_of s1) (do (v_of s2) last2) /\                   
-                   do_pre (concrete_merge (v_of lca) (v_of s1) (do (v_of s2) last2)) last1 /\
+          (ensures //merge_pre (v_of lca) (v_of s1) (do (v_of s2) last2) (*/\                   
+                   //do_pre (concrete_merge (v_of lca) (v_of s1) (do (v_of s2) last2)) last1 /\
                    eq (do (concrete_merge (v_of lca) (v_of s1) (do (v_of s2) last2)) last1)
-                      (concrete_merge (v_of lca) (do (v_of s1) last1) (do (v_of s2) last2))) = ()
+                      (concrete_merge (v_of lca) (do (v_of s1) last1) (do (v_of s2) last2))) = 
+  (*assume ((Remove? (snd last1) /\ Add_after? (snd last2) ==> fst last2 <> get_rem_id last1) /\
+          (Add_after? (snd last1) /\ Add_after? (snd last2) /\ get_after_id last1 <> get_after_id last2 ==>
+                      fst last1 <> get_after_id last2 /\ fst last2 <> get_after_id last1));*)
+  //assume (not (mem_id_s (fst last2) (fst (v_of lca))) /\ not (S.mem (fst last2) (snd (v_of lca))));
+  admit()
 
-let linearizable_gt0_base_stf (lca s1 s2:st) (last1 last2:op_t)
+ let linearizable_gt0_base_stf (lca s1 s2:st) (last1 last2:op_t)
   : Lemma (requires do_pre (v_of s1) last1 /\ do_pre (v_of s2) last2 /\ 
                     consistent_branches lca (do_st s1 last1) (do_st s2 last2) /\
                     consistent_branches lca s1 s2 /\
@@ -277,7 +482,7 @@ let linearizable_gt0_base_stf (lca s1 s2:st) (last1 last2:op_t)
                    eq (do (concrete_merge (v_of lca) (do (v_of s1) last1) (v_of s2)) last2)
                       (concrete_merge (v_of lca) (do (v_of s1) last1) (do (v_of s2) last2))) = ()
 
-let linearizable_gt0_base (lca s1 s2:st) (last1 last2:op_t)
+let linearizable_gt0_base1 (lca s1 s2:st) (last1 last2:op_t)
   : Lemma (requires do_pre (v_of s1) last1 /\ do_pre (v_of s2) last2 /\ 
                     consistent_branches lca (do_st s1 last1) (do_st s2 last2) /\
                     consistent_branches lca s1 s2 /\
@@ -302,7 +507,7 @@ let linearizable_gt0_base (lca s1 s2:st) (last1 last2:op_t)
     linearizable_gt0_base_stf lca s1 s2 last1 last2
   else ()
 
-let linearizable_gt0_s2'_do_pre (lca s1 s2:st) (last1 last2:op_t)
+let linearizable_gt0_s2'_do_pre1 (lca s1 s2:st) (last1 last2:op_t)
   : Lemma (requires do_pre (v_of s1) last1 /\ do_pre (v_of s2) last2 /\ 
                     consistent_branches lca (do_st s1 last1) (do_st s2 last2) /\
                     consistent_branches lca (do_st s1 last1) s2 /\
@@ -311,9 +516,9 @@ let linearizable_gt0_s2'_do_pre (lca s1 s2:st) (last1 last2:op_t)
                     Second_then_first? (resolve_conflict last1 last2)) 
          
           (ensures (length (ops_of s2) > length (ops_of lca) ==> do_pre (v_of (inverse_st s2)) last2) /\
-                   (length (ops_of s1) > length (ops_of lca) ==> do_pre (v_of (inverse_st s1)) last1)) = admit()
+                   (length (ops_of s1) > length (ops_of lca) ==> do_pre (v_of (inverse_st s1)) last1)) = ()
 
-let linearizable_gt0_s2'_merge_pre (lca s1 s2:st) (last1 last2:op_t)
+let linearizable_gt0_s2'_merge_pre1 (lca s1 s2:st) (last1 last2:op_t)
   : Lemma (requires do_pre (v_of s1) last1 /\ do_pre (v_of s2) last2 /\ 
                     consistent_branches lca (do_st s1 last1) (do_st s2 last2) /\
                     consistent_branches lca (do_st s1 last1) s2 /\
@@ -327,7 +532,7 @@ let linearizable_gt0_s2'_merge_pre (lca s1 s2:st) (last1 last2:op_t)
                    (length (ops_of s2) > length (ops_of lca) /\ do_pre (v_of (inverse_st s2)) last2 ==>
                       merge_pre (v_of lca) (do (v_of s1) last1) (do (v_of (inverse_st s2)) last2))) = ()
 
-let linearizable_gt0_s1'_do_pre (lca s1 s2:st) (last1 last2:op_t)
+let linearizable_gt0_s1'_do_pre1 (lca s1 s2:st) (last1 last2:op_t)
   : Lemma (requires do_pre (v_of s1) last1 /\ do_pre (v_of s2) last2 /\ 
                     consistent_branches lca (do_st s1 last1) (do_st s2 last2) /\
                     consistent_branches lca s1 (do_st s2 last2) /\
@@ -336,9 +541,9 @@ let linearizable_gt0_s1'_do_pre (lca s1 s2:st) (last1 last2:op_t)
                     First_then_second? (resolve_conflict last1 last2)) 
          
           (ensures (length (ops_of s2) > length (ops_of lca) ==> do_pre (v_of (inverse_st s2)) last2) /\
-                   (length (ops_of s1) > length (ops_of lca) ==> do_pre (v_of (inverse_st s1)) last1)) = admit()
+                   (length (ops_of s1) > length (ops_of lca) ==> do_pre (v_of (inverse_st s1)) last1)) = ()
 
-let linearizable_gt0_s1'_merge_pre (lca s1 s2:st) (last1 last2:op_t)
+let linearizable_gt0_s1'_merge_pre1 (lca s1 s2:st) (last1 last2:op_t)
   : Lemma (requires do_pre (v_of s1) last1 /\ do_pre (v_of s2) last2 /\ 
                     consistent_branches lca (do_st s1 last1) (do_st s2 last2) /\
                     consistent_branches lca s1 (do_st s2 last2) /\
@@ -352,6 +557,7 @@ let linearizable_gt0_s1'_merge_pre (lca s1 s2:st) (last1 last2:op_t)
                    (length (ops_of s2) > length (ops_of lca) /\ do_pre (v_of (inverse_st s2)) last2 ==>
                       merge_pre (v_of lca) (do (v_of s1) last1) (do (v_of (inverse_st s2)) last2))) = ()
 
+#push-options "--z3rlimit 200"
 let linearizable_gt0_ind_fts (lca s1 s2:st) (last1 last2:op_t)
   : Lemma (requires do_pre (v_of s1) last1 /\ do_pre (v_of s2) last2 /\ 
                     consistent_branches lca (do_st s1 last1) (do_st s2 last2) /\
@@ -362,19 +568,33 @@ let linearizable_gt0_ind_fts (lca s1 s2:st) (last1 last2:op_t)
                     (let s2' = inverse_st s2 in
                     do_pre (v_of s2') last2 /\
                     First_then_second? (resolve_conflict last1 last2) /\
+                    //Remove? (snd last1) /\ Add_after? (snd last2) /\
                     consistent_branches lca s1 (do_st s2' last2) /\
                     consistent_branches lca (do_st s1 last1) (do_st s2' last2) /\
                     consistent_branches lca s1 (do_st s2 last2) /\
                     merge_pre (v_of lca) (v_of s1) (do (v_of s2') last2) /\
                     merge_pre (v_of lca) (do (v_of s1) last1) (do (v_of s2') last2) /\
                     do_pre (concrete_merge (v_of lca) (v_of s1) (do (v_of s2') last2)) last1 /\
+                    merge_pre (v_of lca) (v_of s1) (do (v_of s2) last2) /\
+                    //do_pre (concrete_merge (v_of lca) (v_of s1) (do (v_of s2) last2)) last1 /\
                     eq (do (concrete_merge (v_of lca) (v_of s1) (do (v_of s2') last2)) last1)
                        (concrete_merge (v_of lca) (do (v_of s1) last1) (do (v_of s2') last2)))) 
         
-          (ensures merge_pre (v_of lca) (v_of s1) (do (v_of s2) last2) /\
-                   do_pre (concrete_merge (v_of lca) (v_of s1) (do (v_of s2) last2)) last1 /\
+          (ensures //merge_pre (v_of lca) (v_of s1) (do (v_of s2) last2) ///\
+                   do_pre (concrete_merge (v_of lca) (v_of s1) (do (v_of s2) last2)) last1 (*/\
                    eq (do (concrete_merge (v_of lca) (v_of s1) (do (v_of s2) last2)) last1)
-                      (concrete_merge (v_of lca) (do (v_of s1) last1) (do (v_of s2) last2))) = admit() //only do-pre not done
+                      (concrete_merge (v_of lca) (do (v_of s1) last1) (do (v_of s2) last2)*)) = 
+                      
+  (*assume ((Remove? (snd last1) /\ Add_after? (snd last2) ==> fst last2 <> get_rem_id last1) /\
+          (Add_after? (snd last1) /\ Add_after? (snd last2) /\ get_after_id last1 <> get_after_id last2 ==>
+                      fst last1 <> get_after_id last2 /\ fst last2 <> get_after_id last1));*)
+  lem_apply_log init_st (ops_of s2);
+  let pre, lastop = un_snoc (ops_of s2) in
+  inverse_helper init_st pre lastop; 
+  assume (fst last1 <> fst lastop); //can be done
+  (*if Remove? (snd last1) then () 
+  else 
+    (assert (~ (mem_id_s (fst last1) (fst (concrete_merge (v_of lca) (v_of s1) (do (v_of s2) last2))))); ())*) ()  
                     
 let linearizable_gt0_ind_stf (lca s1 s2:st) (last1 last2:op_t)
   : Lemma (requires do_pre (v_of s1) last1 /\ do_pre (v_of s2) last2 /\ 
@@ -442,13 +662,19 @@ let linearizable_gt0_ind1_stf (lca s1 s2:st) (last1 last2:op_t)
                     merge_pre (v_of lca) (do (v_of s1') last1) (v_of s2) /\
                     merge_pre (v_of lca) (do (v_of s1') last1) (do (v_of s2) last2) /\
                     do_pre (concrete_merge (v_of lca) (do (v_of s1') last1) (v_of s2)) last2 /\
+                    merge_pre (v_of lca) (do (v_of s1) last1) (v_of s2) /\
                     eq (do (concrete_merge (v_of lca) (do (v_of s1') last1) (v_of s2)) last2)
                        (concrete_merge (v_of lca) (do (v_of s1') last1) (do (v_of s2) last2))))
         
-          (ensures merge_pre (v_of lca) (do (v_of s1) last1) (v_of s2) /\
-                   do_pre (concrete_merge (v_of lca) (do (v_of s1) last1) (v_of s2)) last2 /\    
+          (ensures //merge_pre (v_of lca) (do (v_of s1) last1) (v_of s2) (*/\
+                   do_pre (concrete_merge (v_of lca) (do (v_of s1) last1) (v_of s2)) last2 (*/\    
                    eq (do (concrete_merge (v_of lca) (do (v_of s1) last1) (v_of s2)) last2)
-                      (concrete_merge (v_of lca) (do (v_of s1) last1) (do (v_of s2) last2))) = admit() //done except do_pre
+                      (concrete_merge (v_of lca) (do (v_of s1) last1) (do (v_of s2) last2)*)) = 
+  assume ((Add_after? (snd last1) /\ Remove? (snd last2) /\ get_after_id last1 = get_rem_id last2 ==> 
+                      fst last1 <> get_rem_id last2 /\ get_after_id last1 <> fst last2) /\
+          (Add_after? (snd last1) /\ Add_after? (snd last2) /\ get_after_id last1 = get_after_id last2 /\ fst last2 > fst last1 ==>
+                      fst last1 <> get_after_id last2 /\ fst last2 <> get_after_id last1));
+  ()
 
 let fts_merge_pre1 (lca s1 s2:st)
   : Lemma (requires consistent_branches lca s1 s2 /\
@@ -472,7 +698,7 @@ let stf_merge_pre1 (lca s1 s2:st)
                      Second_then_first? (resolve_conflict last1 last2)))
           (ensures merge_pre (v_of lca) (v_of s1) (v_of (inverse_st s2))) = ()
 
-let first_merge_pre1 (lca s1 s2:st)
+(*let first_merge_pre1 (lca s1 s2:st)
   : Lemma (requires consistent_branches lca s1 s2 /\
                     merge_pre (v_of lca) (v_of s1) (v_of s2) /\
                     length (ops_of s1) > length (ops_of lca) /\
@@ -481,7 +707,7 @@ let first_merge_pre1 (lca s1 s2:st)
                      let _, last2 = un_snoc (ops_of s2) in
                      fst last1 <> fst last2 /\
                      First? (resolve_conflict last1 last2)))
-          (ensures merge_pre (v_of lca) (v_of (inverse_st s1)) (v_of (inverse_st s2))) = ()
+          (ensures merge_pre (v_of lca) (v_of (inverse_st s1)) (v_of (inverse_st s2))) = ()*)
 
 let convergence1 (lca s1' s2:concrete_st) (ls1' ls2:log) (o:op_t)
   : Lemma (requires do_pre s1' o /\
